Typecheck.thy
@@ -1,27 +1,28 @@
 theory Typecheck
-imports Vector Expression Kindcheck
+imports Expression Kindcheck
 begin
 
-inductive typecheck :: "nat \<Rightarrow> type list \<Rightarrow> expr \<Rightarrow> type \<Rightarrow> bool" (infix ",_ \<turnstile> _ :" 60) 
-      and typecheck_fs :: "nat \<Rightarrow> type list \<Rightarrow> expr list \<Rightarrow> type list \<Rightarrow> bool" (infix ",_ \<turnstile>\<^sub>f _ :" 60)
-      and typecheck_cs :: "nat \<Rightarrow> type list \<Rightarrow> expr list \<Rightarrow> type list \<Rightarrow> type \<Rightarrow> bool" 
+inductive typecheck :: "kind list \<Rightarrow> type list \<Rightarrow> expr \<Rightarrow> type \<Rightarrow> bool" (infix ",_ \<turnstile> _ :" 60) 
+      and typecheck_fs :: "kind list \<Rightarrow> type list \<Rightarrow> expr list \<Rightarrow> type list \<Rightarrow> bool" 
+    (infix ",_ \<turnstile>\<^sub>f _ :" 60)
+      and typecheck_cs :: "kind list \<Rightarrow> type list \<Rightarrow> expr list \<Rightarrow> type list \<Rightarrow> type \<Rightarrow> bool" 
     (infix ",_ \<turnstile>\<^sub>c _ : _ \<rightarrow>" 60) where
   tc_var [simp]: "lookup x \<Gamma> = Some t \<Longrightarrow> \<Delta>,\<Gamma> \<turnstile> Var x : t"
-| tc_abs [simp]: "\<Delta>,insert_at 0 t\<^sub>1 \<Gamma> \<turnstile> e : t\<^sub>2 \<Longrightarrow> \<Delta> \<turnstile>\<^sub>k t\<^sub>1 \<Longrightarrow> \<Delta>,\<Gamma> \<turnstile> Abs t\<^sub>1 e : Arrow t\<^sub>1 t\<^sub>2"
+| tc_abs [simp]: "\<Delta>,insert_at 0 t\<^sub>1 \<Gamma> \<turnstile> e : t\<^sub>2 \<Longrightarrow> \<Delta> \<turnstile>\<^sub>k t\<^sub>1 : Star \<Longrightarrow> \<Delta>,\<Gamma> \<turnstile> Abs t\<^sub>1 e : Arrow t\<^sub>1 t\<^sub>2"
 | tc_app [simp]: "\<Delta>,\<Gamma> \<turnstile> e\<^sub>1 : Arrow t\<^sub>1 t\<^sub>2 \<Longrightarrow> \<Delta>,\<Gamma> \<turnstile> e\<^sub>2 : t\<^sub>1 \<Longrightarrow> \<Delta>,\<Gamma> \<turnstile> App e\<^sub>1 e\<^sub>2 : t\<^sub>2"
 | tc_let [simp]: "\<Delta>,\<Gamma> \<turnstile> e\<^sub>1 : t\<^sub>1 \<Longrightarrow> \<Delta>,insert_at 0 t\<^sub>1 \<Gamma> \<turnstile> e\<^sub>2 : t\<^sub>2 \<Longrightarrow> \<Delta>,\<Gamma> \<turnstile> Let e\<^sub>1 e\<^sub>2 : t\<^sub>2"
 | tc_rec [simp]: "\<Delta>,\<Gamma> \<turnstile>\<^sub>f fs : ts \<Longrightarrow> \<Delta>,\<Gamma> \<turnstile> Rec fs : Record ts"
 | tc_proj [simp]: "\<Delta>,\<Gamma> \<turnstile> e : Record ts \<Longrightarrow> lookup l ts = Some t \<Longrightarrow> \<Delta>,\<Gamma> \<turnstile> Proj e l : t"
-| tc_inj [simp]: "\<Delta>,\<Gamma> \<turnstile> e : t \<Longrightarrow> lookup l ts = Some t \<Longrightarrow> \<forall>tt \<in> set ts. \<Delta> \<turnstile>\<^sub>k tt \<Longrightarrow> 
+| tc_inj [simp]: "\<Delta>,\<Gamma> \<turnstile> e : t \<Longrightarrow> lookup l ts = Some t \<Longrightarrow> \<forall>tt \<in> set ts. \<Delta> \<turnstile>\<^sub>k tt : Star \<Longrightarrow> 
     \<Delta>,\<Gamma> \<turnstile> Inj l ts e : Variant ts"
 | tc_case [simp]: "\<Delta>,\<Gamma> \<turnstile> e : Variant ts \<Longrightarrow> \<Delta>,\<Gamma> \<turnstile>\<^sub>c cs : ts \<rightarrow> t \<Longrightarrow> \<Delta>,\<Gamma> \<turnstile> Case e t cs : t"
-| tc_fold [simp]: "\<Delta>,\<Gamma> \<turnstile> e : subst\<^sub>t\<^sub>t 0 (Inductive t) t \<Longrightarrow> Suc \<Delta> \<turnstile>\<^sub>k t \<Longrightarrow> 
-    \<Delta>,\<Gamma> \<turnstile> Fold t e : Inductive t"
-| tc_unfold [simp]: "\<Delta>,\<Gamma> \<turnstile> e : Inductive t \<Longrightarrow> Suc \<Delta> \<turnstile>\<^sub>k t \<Longrightarrow> 
-    \<Delta>,\<Gamma> \<turnstile> Unfold t e : subst\<^sub>t\<^sub>t 0 (Inductive t) t"
-| tc_tyabs [simp]: "Suc \<Delta>,map (incr\<^sub>t\<^sub>t 0) \<Gamma> \<turnstile> e : t \<Longrightarrow> \<Delta>,\<Gamma> \<turnstile> TyAbs e : Forall t"
-| tc_tyapp [simp]: "\<Delta>,\<Gamma> \<turnstile> e : Forall t \<Longrightarrow> \<Delta> \<turnstile>\<^sub>k t' \<Longrightarrow> \<Delta>,\<Gamma> \<turnstile> TyApp e t' : subst\<^sub>t\<^sub>t 0 t' t"
-| tc_tylet [simp]: "\<Delta>,\<Gamma> \<turnstile> subst\<^sub>t\<^sub>e 0 t' e : t \<Longrightarrow> \<Delta> \<turnstile>\<^sub>k t' \<Longrightarrow> \<Delta>,\<Gamma> \<turnstile> TyLet t' e : t"
+| tc_fold [simp]: "\<Delta>,\<Gamma> \<turnstile> e : subst\<^sub>t\<^sub>t 0 (Inductive k t) t \<Longrightarrow> insert_at 0 k \<Delta> \<turnstile>\<^sub>k t : Star \<Longrightarrow> 
+    \<Delta>,\<Gamma> \<turnstile> Fold t e : Inductive k t"
+| tc_unfold [simp]: "\<Delta>,\<Gamma> \<turnstile> e : Inductive k t \<Longrightarrow> insert_at 0 k \<Delta> \<turnstile>\<^sub>k t : Star \<Longrightarrow> 
+    \<Delta>,\<Gamma> \<turnstile> Unfold t e : subst\<^sub>t\<^sub>t 0 (Inductive k t) t"
+| tc_tyabs [simp]: "insert_at 0 k \<Delta>,map (incr\<^sub>t\<^sub>t 0) \<Gamma> \<turnstile> e : t \<Longrightarrow> \<Delta>,\<Gamma> \<turnstile> TyAbs k e : Forall k t"
+| tc_tyapp [simp]: "\<Delta>,\<Gamma> \<turnstile> e : Forall k t \<Longrightarrow> \<Delta> \<turnstile>\<^sub>k t' : k \<Longrightarrow> \<Delta>,\<Gamma> \<turnstile> TyApp e t' : subst\<^sub>t\<^sub>t 0 t' t"
+| tc_tylet [simp]: "\<Delta>,\<Gamma> \<turnstile> subst\<^sub>t\<^sub>e 0 t' e : t \<Longrightarrow> \<Delta> \<turnstile>\<^sub>k t' : k \<Longrightarrow> \<Delta>,\<Gamma> \<turnstile> TyLet t' e : t"
 | tcf_nil [simp]: "\<Delta>,\<Gamma> \<turnstile>\<^sub>f [] : []"
 | tcf_cons [simp]: "\<Delta>,\<Gamma> \<turnstile> e : t \<Longrightarrow> \<Delta>,\<Gamma> \<turnstile>\<^sub>f fs : ts \<Longrightarrow> \<Delta>,\<Gamma> \<turnstile>\<^sub>f e # fs : t # ts"
 | tcc_nil [simp]: "\<Delta>,\<Gamma> \<turnstile>\<^sub>c [] : [] \<rightarrow> t"
@@ -38,7 +39,7 @@ inductive_cases [elim]: "\<Delta>,\<Gamma> \<turnstile> Inj e ts l : t"
 inductive_cases [elim]: "\<Delta>,\<Gamma> \<turnstile> Case e tt cs : t"
 inductive_cases [elim]: "\<Delta>,\<Gamma> \<turnstile> Fold t' e : t"
 inductive_cases [elim]: "\<Delta>,\<Gamma> \<turnstile> Unfold t' e : t"
-inductive_cases [elim]: "\<Delta>,\<Gamma> \<turnstile> TyAbs e : t"
+inductive_cases [elim]: "\<Delta>,\<Gamma> \<turnstile> TyAbs k e : t"
 inductive_cases [elim]: "\<Delta>,\<Gamma> \<turnstile> TyApp e t' : t"
 inductive_cases [elim]: "\<Delta>,\<Gamma> \<turnstile> TyLet t' e : t"
 inductive_cases [elim]: "\<Delta>,\<Gamma> \<turnstile>\<^sub>f [] : ts"
@@ -57,12 +58,12 @@ lemma canonical_variant [simp]: "\<Delta>,\<Gamma> \<turnstile> e : Variant ts \
     \<exists>l e'. e = Inj l ts e' \<and> is_value e' \<and> l < length ts"
   by (induction \<Gamma> e "Variant ts" rule: typecheck_typecheck_fs_typecheck_cs.inducts(1)) auto
 
-lemma canonical_inductive [simp]: "\<Delta>,\<Gamma> \<turnstile> e : Inductive t \<Longrightarrow> is_value e \<Longrightarrow> 
+lemma canonical_inductive [simp]: "\<Delta>,\<Gamma> \<turnstile> e : Inductive k t \<Longrightarrow> is_value e \<Longrightarrow> 
     \<exists>e'. e = Fold t e' \<and> is_value e'"
-  by (induction \<Gamma> e "Inductive t" rule: typecheck_typecheck_fs_typecheck_cs.inducts(1)) auto
+  by (induction \<Gamma> e "Inductive k t" rule: typecheck_typecheck_fs_typecheck_cs.inducts(1)) auto
 
-lemma canonical_forall [simp]: "\<Delta>,\<Gamma> \<turnstile> e : Forall t \<Longrightarrow> is_value e \<Longrightarrow> \<exists>e'. e = TyAbs e'"
-  by (induction \<Gamma> e "Forall t" rule: typecheck_typecheck_fs_typecheck_cs.inducts(1)) auto
+lemma canonical_forall [simp]: "\<Delta>,\<Gamma> \<turnstile> e : Forall k t \<Longrightarrow> is_value e \<Longrightarrow> \<exists>e'. e = TyAbs k e'"
+  by (induction \<Gamma> e "Forall k t" rule: typecheck_typecheck_fs_typecheck_cs.inducts(1)) auto
 
 lemma [simp]: "\<Delta>,\<Gamma> \<turnstile>\<^sub>f fs : ts \<Longrightarrow> lookup l ts = Some t \<Longrightarrow> \<exists>e. lookup l fs = Some e"
   by (induction l fs arbitrary: ts rule: lookup.induct) auto
@@ -101,63 +102,79 @@ lemma [simp]: "subst\<^sub>t\<^sub>e x t (incr\<^sub>e\<^sub>e y e) = incr\<^sub
 lemma [simp]: "subst\<^sub>e\<^sub>e x e' (subst\<^sub>t\<^sub>e y t e) = subst\<^sub>t\<^sub>e y t (subst\<^sub>e\<^sub>e x (incr\<^sub>t\<^sub>e y e') e)"
   by (induction e arbitrary: x y t e') simp_all
 
-lemma [simp]: "\<Delta>,\<Gamma> \<turnstile> e : t \<Longrightarrow> Suc \<Delta>,map (incr\<^sub>t\<^sub>t x) \<Gamma> \<turnstile> incr\<^sub>t\<^sub>e x e : incr\<^sub>t\<^sub>t x t"
-  and [simp]: "\<Delta>,\<Gamma> \<turnstile>\<^sub>f fs : ts \<Longrightarrow> Suc \<Delta>,map (incr\<^sub>t\<^sub>t x) \<Gamma> \<turnstile>\<^sub>f map (incr\<^sub>t\<^sub>e x) fs : map (incr\<^sub>t\<^sub>t x) ts"
-  and [simp]: "\<Delta>,\<Gamma> \<turnstile>\<^sub>c cs : ts \<rightarrow> t \<Longrightarrow>
-    Suc \<Delta>,map (incr\<^sub>t\<^sub>t x) \<Gamma> \<turnstile>\<^sub>c map (incr\<^sub>t\<^sub>e x) cs : map (incr\<^sub>t\<^sub>t x) ts \<rightarrow> incr\<^sub>t\<^sub>t x t "
+lemma [simp]: "\<Delta>,\<Gamma> \<turnstile> e : t \<Longrightarrow> x \<le> length \<Delta> \<Longrightarrow> 
+    insert_at x k \<Delta>,map (incr\<^sub>t\<^sub>t x) \<Gamma> \<turnstile> incr\<^sub>t\<^sub>e x e : incr\<^sub>t\<^sub>t x t"
+  and [simp]: "\<Delta>,\<Gamma> \<turnstile>\<^sub>f fs : ts \<Longrightarrow> x \<le> length \<Delta> \<Longrightarrow> 
+    insert_at x k \<Delta>,map (incr\<^sub>t\<^sub>t x) \<Gamma> \<turnstile>\<^sub>f map (incr\<^sub>t\<^sub>e x) fs : map (incr\<^sub>t\<^sub>t x) ts"
+  and [simp]: "\<Delta>,\<Gamma> \<turnstile>\<^sub>c cs : ts \<rightarrow> t \<Longrightarrow> x \<le> length \<Delta> \<Longrightarrow> 
+    insert_at x k \<Delta>,map (incr\<^sub>t\<^sub>t x) \<Gamma> \<turnstile>\<^sub>c map (incr\<^sub>t\<^sub>e x) cs : map (incr\<^sub>t\<^sub>t x) ts \<rightarrow> incr\<^sub>t\<^sub>t x t "
   proof (induction \<Delta> \<Gamma> e t and \<Delta> \<Gamma> fs ts and \<Delta> \<Gamma> cs ts t arbitrary: x and x and x
          rule: typecheck_typecheck_fs_typecheck_cs.inducts) 
   case (tc_app \<Delta> \<Gamma> e\<^sub>1 t\<^sub>1 t\<^sub>2 e\<^sub>2)
-    hence "Suc \<Delta>,map (incr\<^sub>t\<^sub>t x) \<Gamma> \<turnstile> incr\<^sub>t\<^sub>e x e\<^sub>1 : Arrow (incr\<^sub>t\<^sub>t x t\<^sub>1) (incr\<^sub>t\<^sub>t x t\<^sub>2)" by simp
-    moreover from tc_app have "Suc \<Delta>,map (incr\<^sub>t\<^sub>t x) \<Gamma> \<turnstile> incr\<^sub>t\<^sub>e x e\<^sub>2 : incr\<^sub>t\<^sub>t x t\<^sub>1" by simp
+    hence "insert_at x k \<Delta>,map (incr\<^sub>t\<^sub>t x) \<Gamma> \<turnstile> incr\<^sub>t\<^sub>e x e\<^sub>1 : Arrow (incr\<^sub>t\<^sub>t x t\<^sub>1) (incr\<^sub>t\<^sub>t x t\<^sub>2)" by simp
+    moreover from tc_app have "insert_at x k \<Delta>,map (incr\<^sub>t\<^sub>t x) \<Gamma> \<turnstile> incr\<^sub>t\<^sub>e x e\<^sub>2 : incr\<^sub>t\<^sub>t x t\<^sub>1" by simp
     ultimately show ?case by simp
   next case (tc_let \<Delta> \<Gamma> e\<^sub>1 t\<^sub>1 e\<^sub>2 t\<^sub>2)
-    hence "Suc \<Delta>,insert_at 0 (incr\<^sub>t\<^sub>t x t\<^sub>1) (map (incr\<^sub>t\<^sub>t x) \<Gamma>) \<turnstile> incr\<^sub>t\<^sub>e x e\<^sub>2 : incr\<^sub>t\<^sub>t x t\<^sub>2" by simp
-    moreover from tc_let have "Suc \<Delta>,map (incr\<^sub>t\<^sub>t x) \<Gamma> \<turnstile> incr\<^sub>t\<^sub>e x e\<^sub>1 : incr\<^sub>t\<^sub>t x t\<^sub>1" by simp
+    hence "insert_at x k \<Delta>,insert_at 0 (incr\<^sub>t\<^sub>t x t\<^sub>1) (map (incr\<^sub>t\<^sub>t x) \<Gamma>) \<turnstile> incr\<^sub>t\<^sub>e x e\<^sub>2 : incr\<^sub>t\<^sub>t x t\<^sub>2" 
+      by simp
+    moreover from tc_let have "insert_at x k \<Delta>,map (incr\<^sub>t\<^sub>t x) \<Gamma> \<turnstile> incr\<^sub>t\<^sub>e x e\<^sub>1 : incr\<^sub>t\<^sub>t x t\<^sub>1" by simp
     ultimately show ?case by simp
   next case (tc_proj \<Delta> \<Gamma> e ts l t)
-    hence "Suc \<Delta>,map (incr\<^sub>t\<^sub>t x) \<Gamma> \<turnstile> incr\<^sub>t\<^sub>e x e : Record (map (incr\<^sub>t\<^sub>t x) ts)" by simp
+    hence "insert_at x k \<Delta>,map (incr\<^sub>t\<^sub>t x) \<Gamma> \<turnstile> incr\<^sub>t\<^sub>e x e : Record (map (incr\<^sub>t\<^sub>t x) ts)" by simp
     moreover from tc_proj have "lookup l (map (incr\<^sub>t\<^sub>t x) ts) = Some (incr\<^sub>t\<^sub>t x t)" by simp
     ultimately show ?case by simp
   next case (tc_inj \<Delta> \<Gamma> e t l ts)
-    hence "Suc \<Delta>,map (incr\<^sub>t\<^sub>t x) \<Gamma> \<turnstile> incr\<^sub>t\<^sub>e x e : incr\<^sub>t\<^sub>t x t" by simp
+    hence "insert_at x k \<Delta>,map (incr\<^sub>t\<^sub>t x) \<Gamma> \<turnstile> incr\<^sub>t\<^sub>e x e : incr\<^sub>t\<^sub>t x t" by simp
     moreover from tc_inj have "lookup l (map (incr\<^sub>t\<^sub>t x) ts) = Some (incr\<^sub>t\<^sub>t x t)" by simp
-    moreover from tc_inj have "\<forall>tt \<in> set (map (incr\<^sub>t\<^sub>t x) ts). Suc \<Delta> \<turnstile>\<^sub>k tt" by simp
+    moreover from tc_inj have "\<forall>tt \<in> set (map (incr\<^sub>t\<^sub>t x) ts). insert_at x k \<Delta> \<turnstile>\<^sub>k tt : Star" by simp
     ultimately show ?case by simp
   next case (tc_case \<Delta> \<Gamma> e ts cs t)
-    hence "Suc \<Delta>,map (incr\<^sub>t\<^sub>t x) \<Gamma> \<turnstile> incr\<^sub>t\<^sub>e x e : Variant (map (incr\<^sub>t\<^sub>t x) ts)" by simp
-    moreover from tc_case have "Suc \<Delta>,map (incr\<^sub>t\<^sub>t x) \<Gamma> \<turnstile>\<^sub>c map (incr\<^sub>t\<^sub>e x) cs : 
+    hence "insert_at x k \<Delta>,map (incr\<^sub>t\<^sub>t x) \<Gamma> \<turnstile> incr\<^sub>t\<^sub>e x e : Variant (map (incr\<^sub>t\<^sub>t x) ts)" by simp
+    moreover from tc_case have "insert_at x k \<Delta>,map (incr\<^sub>t\<^sub>t x) \<Gamma> \<turnstile>\<^sub>c map (incr\<^sub>t\<^sub>e x) cs : 
       map (incr\<^sub>t\<^sub>t x) ts \<rightarrow> incr\<^sub>t\<^sub>t x t" by simp
     ultimately show ?case by simp
-  next case (tc_fold \<Delta> \<Gamma> e t)
-    hence "Suc \<Delta>,map (incr\<^sub>t\<^sub>t x) \<Gamma> \<turnstile> incr\<^sub>t\<^sub>e x e : 
-      subst\<^sub>t\<^sub>t 0 (incr\<^sub>t\<^sub>t x (Inductive t)) (incr\<^sub>t\<^sub>t (Suc x) t)" by (metis le0 subst_incr_swap)
+  next case (tc_fold \<Delta> \<Gamma> e k' t)
+    hence "insert_at x k \<Delta>,map (incr\<^sub>t\<^sub>t x) \<Gamma> \<turnstile> incr\<^sub>t\<^sub>e x e : 
+      subst\<^sub>t\<^sub>t 0 (incr\<^sub>t\<^sub>t x (Inductive k' t)) (incr\<^sub>t\<^sub>t (Suc x) t)" by (metis le0 subst_incr_swap)
     with tc_fold show ?case by simp
-  next case (tc_unfold \<Delta> \<Gamma> e t)
-    hence "Suc \<Delta>,map (incr\<^sub>t\<^sub>t x) \<Gamma> \<turnstile> Unfold (incr\<^sub>t\<^sub>t (Suc x) t) (incr\<^sub>t\<^sub>e x e) : 
-      subst\<^sub>t\<^sub>t 0 (incr\<^sub>t\<^sub>t x (Inductive t)) (incr\<^sub>t\<^sub>t (Suc x) t)" by simp
-    hence "Suc \<Delta>,map (incr\<^sub>t\<^sub>t x) \<Gamma> \<turnstile> Unfold (incr\<^sub>t\<^sub>t (Suc x) t) (incr\<^sub>t\<^sub>e x e) : 
-      incr\<^sub>t\<^sub>t x (subst\<^sub>t\<^sub>t 0 (Inductive t) t)" by (metis le0 subst_incr_swap)
+  next case (tc_unfold \<Delta> \<Gamma> e k' t)
+    hence "insert_at x k \<Delta>,map (incr\<^sub>t\<^sub>t x) \<Gamma> \<turnstile> Unfold (incr\<^sub>t\<^sub>t (Suc x) t) (incr\<^sub>t\<^sub>e x e) : 
+      subst\<^sub>t\<^sub>t 0 (incr\<^sub>t\<^sub>t x (Inductive k' t)) (incr\<^sub>t\<^sub>t (Suc x) t)" by simp
+    hence "insert_at x k \<Delta>,map (incr\<^sub>t\<^sub>t x) \<Gamma> \<turnstile> Unfold (incr\<^sub>t\<^sub>t (Suc x) t) (incr\<^sub>t\<^sub>e x e) : 
+      incr\<^sub>t\<^sub>t x (subst\<^sub>t\<^sub>t 0 (Inductive k' t) t)" by (metis le0 subst_incr_swap)
     thus ?case by simp
-  next case (tc_tyapp \<Delta> \<Gamma> e t t')
-    hence "Suc \<Delta>,map (incr\<^sub>t\<^sub>t x) \<Gamma> \<turnstile> incr\<^sub>t\<^sub>e x e : Forall (incr\<^sub>t\<^sub>t (Suc x) t)" by simp 
-    moreover from tc_tyapp have "Suc \<Delta> \<turnstile>\<^sub>k incr\<^sub>t\<^sub>t x t'" by simp
-    ultimately have "Suc \<Delta>,map (incr\<^sub>t\<^sub>t x) \<Gamma> \<turnstile> TyApp (incr\<^sub>t\<^sub>e x e) (incr\<^sub>t\<^sub>t x t') : 
+  next case (tc_tyapp \<Delta> \<Gamma> e k' t t')
+    hence "insert_at x k \<Delta>,map (incr\<^sub>t\<^sub>t x) \<Gamma> \<turnstile> incr\<^sub>t\<^sub>e x e : Forall k' (incr\<^sub>t\<^sub>t (Suc x) t)" by simp 
+    moreover from tc_tyapp have "insert_at x k \<Delta> \<turnstile>\<^sub>k incr\<^sub>t\<^sub>t x t' : k'" by simp
+    ultimately have "insert_at x k \<Delta>,map (incr\<^sub>t\<^sub>t x) \<Gamma> \<turnstile> TyApp (incr\<^sub>t\<^sub>e x e) (incr\<^sub>t\<^sub>t x t') : 
       subst\<^sub>t\<^sub>t 0 (incr\<^sub>t\<^sub>t x t') (incr\<^sub>t\<^sub>t (Suc x) t)"
         by (metis typecheck_typecheck_fs_typecheck_cs.tc_tyapp)
     thus ?case by simp
+  next case (tc_tylet \<Delta> \<Gamma> t' e t k')
+    hence "insert_at x k \<Delta>,map (incr\<^sub>t\<^sub>t x) \<Gamma> \<turnstile> subst\<^sub>t\<^sub>e 0 (incr\<^sub>t\<^sub>t x t') (incr\<^sub>t\<^sub>e (Suc x) e) : incr\<^sub>t\<^sub>t x t" 
+      by simp
+    moreover from tc_tylet have "insert_at x k \<Delta> \<turnstile>\<^sub>k incr\<^sub>t\<^sub>t x t' : k'" by simp
+    ultimately show ?case by simp
   qed simp_all
 
-lemma tc_subst\<^sub>t\<^sub>e [simp]: "Suc \<Delta>,\<Gamma> \<turnstile> e : t \<Longrightarrow> \<Delta> \<turnstile>\<^sub>k t' \<Longrightarrow> x \<le> \<Delta> \<Longrightarrow> 
+lemma tc_subst\<^sub>t\<^sub>e [simp]: "insert_at x k \<Delta>,\<Gamma> \<turnstile> e : t \<Longrightarrow> \<Delta> \<turnstile>\<^sub>k t' : k \<Longrightarrow> x \<le> length \<Delta> \<Longrightarrow> 
     \<Delta>,map (subst\<^sub>t\<^sub>t x t') \<Gamma> \<turnstile> subst\<^sub>t\<^sub>e x t' e : subst\<^sub>t\<^sub>t x t' t"
-  and [simp]: "Suc \<Delta>,\<Gamma> \<turnstile>\<^sub>f fs : ts \<Longrightarrow> \<Delta> \<turnstile>\<^sub>k t' \<Longrightarrow> x \<le> \<Delta> \<Longrightarrow> 
+  and [simp]: "insert_at x k \<Delta>,\<Gamma> \<turnstile>\<^sub>f fs : ts \<Longrightarrow> \<Delta> \<turnstile>\<^sub>k t' : k \<Longrightarrow> x \<le> length \<Delta> \<Longrightarrow> 
     \<Delta>,map (subst\<^sub>t\<^sub>t x t') \<Gamma> \<turnstile>\<^sub>f map (subst\<^sub>t\<^sub>e x t') fs : map (subst\<^sub>t\<^sub>t x t') ts"
-  and [simp]: "Suc \<Delta>,\<Gamma> \<turnstile>\<^sub>c cs : ts \<rightarrow> t \<Longrightarrow> \<Delta> \<turnstile>\<^sub>k t' \<Longrightarrow> x \<le> \<Delta> \<Longrightarrow> 
+  and [simp]: "insert_at x k \<Delta>,\<Gamma> \<turnstile>\<^sub>c cs : ts \<rightarrow> t \<Longrightarrow> \<Delta> \<turnstile>\<^sub>k t' : k \<Longrightarrow> x \<le> length \<Delta> \<Longrightarrow> 
     \<Delta>,map (subst\<^sub>t\<^sub>t x t') \<Gamma> \<turnstile>\<^sub>c map (subst\<^sub>t\<^sub>e x t') cs : map (subst\<^sub>t\<^sub>t x t') ts \<rightarrow> subst\<^sub>t\<^sub>t x t' t "
-  by (induction "Suc \<Delta>" \<Gamma> e t and "Suc \<Delta>" \<Gamma> fs ts and "Suc \<Delta>" \<Gamma> cs ts t 
-      arbitrary: \<Delta> x t' and \<Delta> x t' and \<Delta> x t'
-      rule: typecheck_typecheck_fs_typecheck_cs.inducts) 
-     fastforce+
+  proof (induction "insert_at x k \<Delta>" \<Gamma> e t and "insert_at x k \<Delta>" \<Gamma> fs ts and "insert_at x k \<Delta>" \<Gamma> cs ts t 
+         arbitrary: \<Delta> x t' and \<Delta> x t' and \<Delta> x t'
+         rule: typecheck_typecheck_fs_typecheck_cs.inducts) 
+  case (tc_inj \<Gamma> e t l ts)
+    moreover hence "\<forall>tt \<in> set (map (subst\<^sub>t\<^sub>t x t') ts). \<Delta> \<turnstile>\<^sub>k tt : Star" by fastforce
+    ultimately show ?case by fastforce
+  next case (tc_tylet \<Gamma> tt e t k)
+    hence "\<Delta>,map (subst\<^sub>t\<^sub>t x t') \<Gamma> \<turnstile> subst\<^sub>t\<^sub>e 0 (subst\<^sub>t\<^sub>t x t' tt) (subst\<^sub>t\<^sub>e (Suc x) (incr\<^sub>t\<^sub>t 0 t') e) : 
+      subst\<^sub>t\<^sub>t x t' t" by simp
+    moreover from tc_tylet have "\<Delta> \<turnstile>\<^sub>k subst\<^sub>t\<^sub>t x t' tt : k" by simp
+    ultimately show ?case by simp
+  qed fastforce+
 
 lemma [simp]: "\<Delta>,\<Gamma> \<turnstile> e : t \<Longrightarrow> x \<le> length \<Gamma> \<Longrightarrow> \<Delta>,insert_at x t' \<Gamma> \<turnstile> incr\<^sub>e\<^sub>e x e : t"
   and [simp]: "\<Delta>,\<Gamma> \<turnstile>\<^sub>f fs : ts \<Longrightarrow> x \<le> length \<Gamma> \<Longrightarrow> \<Delta>,insert_at x t' \<Gamma> \<turnstile>\<^sub>f map (incr\<^sub>e\<^sub>e x) fs : ts"
@@ -180,12 +197,15 @@ lemma [simp]: "\<Delta>,\<Gamma> \<turnstile> e : t \<Longrightarrow> x \<le> le
   next case (tc_inj \<Delta> \<Gamma> e t l ts)
     hence "\<Delta>,insert_at x t' \<Gamma> \<turnstile> incr\<^sub>e\<^sub>e x e : t" by simp
     moreover from tc_inj have "lookup l ts = Some t" by simp
-    moreover from tc_inj have "\<forall>tt \<in> set ts. \<Delta> \<turnstile>\<^sub>k tt" by simp
+    moreover from tc_inj have "\<forall>tt \<in> set ts. \<Delta> \<turnstile>\<^sub>k tt : Star" by simp
     ultimately show ?case by simp
   next case (tc_case \<Delta> \<Gamma> e ts cs t)
     hence "\<Delta>,insert_at x t' \<Gamma> \<turnstile> incr\<^sub>e\<^sub>e x e : Variant ts " by simp
     moreover from tc_case have "\<Delta>,insert_at x t' \<Gamma> \<turnstile>\<^sub>c map (incr\<^sub>e\<^sub>e (Suc x)) cs : ts \<rightarrow> t" by simp
     ultimately show ?case by simp
+  next case (tc_tyapp \<Delta> \<Gamma> e k t tt)
+    moreover hence "\<Delta>,insert_at x t' \<Gamma> \<turnstile> incr\<^sub>e\<^sub>e x e : Forall k t" by simp 
+    ultimately show ?case by fastforce
   qed simp_all
 
 lemma [simp]: "\<Delta>,insert_at x t' \<Gamma> \<turnstile> e : t \<Longrightarrow> x \<le> length \<Gamma> \<Longrightarrow> \<Delta>,\<Gamma> \<turnstile> e' : t' \<Longrightarrow> 
