Evaluate.thy
@@ -8,7 +8,7 @@ inductive reduce :: "expr \<Rightarrow> expr \<Rightarrow> bool" (infix "\<leads
 | ev_proj [simp]: "is_value_f fs \<Longrightarrow> lookup l fs = Some e \<Longrightarrow> Proj (Rec fs) l \<leadsto>\<^sub>\<beta> e" 
 | ev_case [simp]: "is_value e \<Longrightarrow> lookup l cs = Some e' \<Longrightarrow> Case (Inj l ts e) t cs \<leadsto>\<^sub>\<beta> subst\<^sub>e\<^sub>e 0 e e'" 
 | ev_fold [simp]: "is_value e \<Longrightarrow> Unfold t (Fold t e) \<leadsto>\<^sub>\<beta> e" 
-| ev_tbeta [simp]: "TyApp (TyAbs e) t \<leadsto>\<^sub>\<beta> subst\<^sub>t\<^sub>e 0 t e" 
+| ev_tbeta [simp]: "TyApp (TyAbs k e) t \<leadsto>\<^sub>\<beta> subst\<^sub>t\<^sub>e 0 t e" 
 | ev_tlet [simp]: "TyLet t e \<leadsto>\<^sub>\<beta> subst\<^sub>t\<^sub>e 0 t e" 
 
 inductive evaluate :: "expr \<Rightarrow> expr \<Rightarrow> bool" (infix "\<leadsto>" 60) where
@@ -54,12 +54,12 @@ theorem [simp]: "\<Delta>,[] \<turnstile> e : t \<Longrightarrow> unfold e = (s,
     thus ?case
       proof (cases "is_value e")
       case True
-        with tc_case obtain l e' where E: "r = Case (Inj l ts e') t cs \<and> is_value e' \<and> l < length ts" 
-          by fastforce
+        with tc_case obtain l e' where E: "r = Case (Inj l ts e') t cs \<and> is_value e' \<and> 
+          l < length ts" by fastforce
         moreover with tc_case obtain r' where "lookup l cs = Some r'" by fastforce
         ultimately show ?thesis using ev_case by blast
       qed (auto split: prod.splits)
-  next case (tc_unfold \<Delta> e t)
+  next case (tc_unfold \<Delta> e k t)
     thus ?case
       proof (cases "is_value e")
       case True
@@ -67,11 +67,11 @@ theorem [simp]: "\<Delta>,[] \<turnstile> e : t \<Longrightarrow> unfold e = (s,
         hence "r \<leadsto>\<^sub>\<beta> e'" by simp
         thus ?thesis by blast
       qed (auto split: prod.splits)
-  next case (tc_tyapp \<Delta> e t t')
+  next case (tc_tyapp \<Delta> e k t t')
     thus ?case
       proof (cases "is_value e")
       case True
-        with tc_tyapp obtain e' where "e = TyAbs e'" by fastforce
+        with tc_tyapp obtain e' where "e = TyAbs k e'" by fastforce
         with tc_tyapp True have "r \<leadsto>\<^sub>\<beta> subst\<^sub>t\<^sub>e 0 t' e'" by fastforce
         thus ?thesis by fastforce
       qed (auto split: prod.splits)
@@ -97,13 +97,13 @@ theorem progress: "\<Delta>,[] \<turnstile> e : t \<Longrightarrow> is_value e \
 lemma preservation\<^sub>\<beta>: "e \<leadsto>\<^sub>\<beta> e' \<Longrightarrow> \<Delta>,\<Gamma> \<turnstile> e : t \<Longrightarrow> \<Delta>,\<Gamma> \<turnstile> e' : t"
   proof (induction e e' rule: reduce.induct) 
   case (ev_case e l cs e' ts tt)
-    then obtain t' where "(\<Delta>,\<Gamma> \<turnstile> e : t') \<and> lookup l ts = Some t' \<and> (\<forall>tt \<in> set ts. \<Delta> \<turnstile>\<^sub>k tt) \<and> 
-      (\<Delta>,\<Gamma> \<turnstile>\<^sub>c cs : ts \<rightarrow> t) \<and> t = tt" by fastforce
+    then obtain t' where "(\<Delta>,\<Gamma> \<turnstile> e : t') \<and> lookup l ts = Some t' \<and> 
+      (\<forall>tt \<in> set ts. \<Delta> \<turnstile>\<^sub>k tt : Star) \<and> (\<Delta>,\<Gamma> \<turnstile>\<^sub>c cs : ts \<rightarrow> t) \<and> t = tt" by fastforce
     moreover with ev_case have "\<Delta>,insert_at 0 t' \<Gamma> \<turnstile> e' : t" by fastforce
     ultimately show ?case by simp
-  next case (ev_tbeta e t')
-    then obtain tt where "(Suc \<Delta>,map (incr\<^sub>t\<^sub>t 0) \<Gamma> \<turnstile> e : tt) \<and> (\<Delta> \<turnstile>\<^sub>k t') \<and> t = subst\<^sub>t\<^sub>t 0 t' tt" 
-      by fastforce
+  next case (ev_tbeta k e t')
+    then obtain tt where "(insert_at 0 k \<Delta>,map (incr\<^sub>t\<^sub>t 0) \<Gamma> \<turnstile> e : tt) \<and> (\<Delta> \<turnstile>\<^sub>k t' : k) \<and> 
+      t = subst\<^sub>t\<^sub>t 0 t' tt" by fastforce
     hence "\<Delta>,map (subst\<^sub>t\<^sub>t 0 t') (map (incr\<^sub>t\<^sub>t 0) \<Gamma>) \<turnstile> subst\<^sub>t\<^sub>e 0 t' e : t" using tc_subst\<^sub>t\<^sub>e by blast
     thus ?case by simp
   qed fastforce+
